coq/Subs2.v
@@ -1,0 +1,142 @@
+Require Import Coq.Arith.EqNat.
+Require Import Coq.Lists.List.
+Require Import Coq.Bool.Bool.
+Require Import Coq.Classes.RelationClasses.
+Require Import Coq.Setoids.Setoid Coq.Classes.SetoidClass.
+Require Import Cases.
+Require Import Term2.
+Require Import Env.
+
+Module ValueImpl <: VALUE.
+  Definition val := term.
+End ValueImpl.
+
+Module VarImpl <: VARIABLE.
+  Definition var := var.
+  Definition beq_var := beq_var.
+
+  Definition beq_var_refl := beq_var_refl.
+  Definition beq_var_sym := beq_var_sym.
+  Definition beq_var_trans := beq_var_trans.
+End VarImpl.
+
+Module StdEnv := ENV(ValueImpl)(VarImpl).
+Import StdEnv.
+
+Definition try_lookup v a :=
+  match lookup v a with
+    | None => tvar v
+    | Some p => p
+  end.
+
+Fixpoint subs a p : term :=
+  match p with
+    | tvar v => try_lookup v a
+    | const c => const c
+    | empty => empty
+    | cons p ps => cons (subs a p) (subs a ps)
+  end.
+
+Notation "a * p" := (subs a p).
+
+Definition env_eqv a b :=
+  forall (v : var), try_lookup v a = try_lookup v b.
+
+
+Lemma env_eqv_refl : forall a, env_eqv a a.
+Proof. unfold env_eqv. reflexivity. Qed.
+Lemma env_eqv_sym : forall a b, env_eqv a b -> env_eqv b a.
+Proof. unfold env_eqv. intros. symmetry; auto. Qed.
+Lemma env_eqv_trans : forall a b c, env_eqv a b -> env_eqv b c -> env_eqv a c.
+Proof. unfold env_eqv. intros. rewrite H; auto. Qed.
+
+Add Relation env env_eqv
+  reflexivity proved by env_eqv_refl
+  symmetry proved by env_eqv_sym
+  transitivity proved by env_eqv_trans
+    as Env_eqv.
+
+Instance env_eqv_Setoid : Setoid env :=
+  {equiv := env_eqv; setoid_equiv := Env_eqv}.
+
+
+Lemma lookup_eqv : forall v a b,
+  lookup v a = lookup v b -> try_lookup v a = try_lookup v b.
+Proof.
+  intros. unfold try_lookup. rewrite H. reflexivity.
+Qed.
+Hint Resolve lookup_eqv.
+
+Lemma env_eqv_subs : forall a b p,
+  a == b -> a * p = b * p.
+Proof.
+  intros. induction p; auto.
+  Case "var v". simpl. unfold env_eqv in H.
+    rewrite H. reflexivity.
+  Case "cons p1 p2".
+    simpl. rewrite IHp1. rewrite IHp2. reflexivity.
+Qed.
+
+Lemma subs_mtEnv : forall p, mtEnv * p = p.
+Proof.
+  intros. induction p; try reflexivity.
+  Case "cons p1 p2".
+    simpl. rewrite IHp1. rewrite IHp2. reflexivity.
+Qed.
+
+Lemma try_lookup_not_mem : forall v a,
+  mem v a = false -> try_lookup v a = tvar v.
+Proof.
+  intros. assert (G : lookup v a = None).
+    apply lookup_not_mem. exact H.
+  unfold try_lookup. rewrite G. reflexivity.
+Qed.
+Hint Resolve try_lookup_not_mem.
+
+Fixpoint compose (a b : env) : env :=
+  match b with
+    | mtEnv => a
+    | bind v t b => bind v (a * t) (compose a b)
+  end.
+
+Lemma compose_mtEnv_l : forall a, compose mtEnv a = a.
+Proof.
+  intros. induction a; try reflexivity.
+  simpl. rewrite IHa. rewrite subs_mtEnv. reflexivity.
+Qed.
+
+Add Parametric Morphism : subs with signature (equiv ==> eq ==> eq) as Subs_morph.
+Proof.
+  intros. apply env_eqv_subs. assumption.
+Qed.
+
+Lemma compose_subs_eq : forall a b p,
+  a * (b * p) = (compose a b) * p.
+Proof.
+  intros.
+  induction p; auto.
+  Case "t = var v".
+    simpl. induction b as [|v2 p2 b].
+    SCase "b = mtEnv".
+      reflexivity.
+    SCase "b = bind v2 p2 b".
+      simpl. unfold try_lookup, lookup.
+      destruct (VarImpl.beq_var v v2); auto.
+  Case "t = cons p1 p2".
+    simpl. rewrite IHp1, IHp2. reflexivity.
+Qed.
+
+Lemma subs_lookup_eqv : forall a b,
+  a == b <-> forall p, a * p = b * p.
+Proof.
+  intros. simpl. unfold env_eqv.
+  split; intros.
+  Case "a == b -> at = bt".
+    induction p; auto.
+    SCase "t = tvar v".
+      simpl. apply H.
+    SCase "t = cons p1 p2".
+      simpl. rewrite IHp1, IHp2. reflexivity.
+  Case "at = bt -> a == b".
+    specialize H with (tvar v). simpl in H. exact H.
+Qed.
