coq/Term2.v
@@ -1,0 +1,55 @@
+Require Import Coq.Arith.EqNat.
+Require Import Coq.Bool.Bool.
+
+
+Definition var := nat.
+Definition id := nat.
+Definition beq_var := beq_nat.
+Definition beq_id := beq_nat.
+
+Inductive term :=
+| tvar : var -> term
+| const : id -> term
+| empty : term
+| cons : term -> term -> term.
+
+
+Fixpoint fvar v p : bool :=
+  match p with
+    | tvar v' => beq_var v v'
+    | const c => false
+    | empty => false
+    | cons p ps => fvar v p || fvar v ps
+  end.
+
+Definition closed p : Prop :=
+  forall (v : var), fvar v p = false.
+
+Lemma beq_var_refl : forall (x : var),
+  beq_var x x = true.
+Proof. intro. rewrite <- beq_nat_refl. reflexivity. Qed.
+Hint Resolve beq_var_refl.
+
+Lemma beq_var_sym : forall (x y : var),
+  beq_var x y = beq_var y x.
+Proof.
+  induction x; induction y; auto.
+  simpl. apply IHx.
+Qed.
+
+Lemma beq_var_trans : forall (x y z : var),
+  beq_var x y = true -> beq_var y z = true -> beq_var x z = true.
+Proof.
+  intros. unfold beq_var in *.
+  apply beq_nat_true in H. rewrite H. exact H0.
+Qed.
+
+Lemma beq_var_true : forall x y : var, beq_var x y = true -> x = y.
+Proof. intros. apply beq_nat_true. assumption. Qed.
+
+Lemma beq_id_refl : forall (n : id), beq_id n n = true.
+Proof. intros. rewrite (beq_nat_refl n). reflexivity. Qed.
+Hint Resolve beq_id_refl.
+
+Lemma beq_id_true : forall x y : id, beq_id x y = true -> x = y.
+Proof. intros. apply beq_nat_true. assumption. Qed.
