coq/TermFaithful.v
@@ -1,0 +1,158 @@
+Require Import Coq.Lists.List.
+Require Import Coq.Arith.EqNat.
+Require Import Cases.
+Require Import Term2.
+Require Import Env.
+
+Unset Elimination Schemes.
+Inductive lterm :=
+| lvar : var -> lterm
+| lnode : id -> list lterm -> lterm.
+Set Elimination Schemes.
+
+Definition lterm_rect := fun
+  (P : lterm -> Type)
+  (h : forall (v : var), P (lvar v))
+  (g : forall (n : id), P (lnode n nil))
+  (f : forall (n : id) (t : lterm) (ts : list lterm),
+    P t -> P (lnode n ts) -> P (lnode n (t :: ts)))
+  =>
+  fix lterm_rec (t : lterm) : P t :=
+  match t return P t with
+    | lvar v => h v
+    | lnode n ts =>
+      ((fix lterms_rec (ts : list lterm) : P (lnode n ts) :=
+        match ts with
+          | nil => g n
+          | t :: ts => f n t ts (lterm_rec t) (lterms_rec ts)
+        end) ts)
+  end.
+
+Definition lterm_ind := fun
+  (P : lterm -> Prop)
+  (h : forall (v : var), P (lvar v))
+  (g : forall (n : id), P (lnode n nil))
+  (f : forall (n : id) (t : lterm) (ts : list lterm),
+    P t -> P (lnode n ts) -> P (lnode n (t :: ts)))
+  => lterm_rect P h g f.
+
+Definition lterm_rec := fun
+  (P : lterm -> Set)
+  (h : forall (v : var), P (lvar v))
+  (g : forall (n : id), P (lnode n nil))
+  (f : forall (n : id) (t : lterm) (ts : list lterm),
+    P t -> P (lnode n ts) -> P (lnode n (t :: ts)))
+  => lterm_rect P h g f.
+
+Module Type VALUE.
+  Parameter val : Type.
+End VALUE.
+
+(*
+Module ENV (Import Value : VALUE).
+
+  Inductive env :=
+  | mtEnv : env
+  | bind : var -> val -> env -> env.
+
+  Fixpoint lookup (v : var) (e : env) : option val :=
+    match e with
+      | mtEnv => None
+      | bind v' t e =>
+        if beq_nat v v'
+          then Some t
+          else lookup v e
+    end.
+End ENV.
+*)
+Module ValueM <: VALUE.
+  Definition val := lterm.
+End ValueM.
+Module VarM <: VARIABLE.
+  Definition var := var.
+  Definition beq_var := beq_var.
+  Definition beq_var_refl := beq_var_refl.
+  Definition beq_var_sym := beq_var_sym.
+  Definition beq_var_trans := beq_var_trans.
+End VarM.
+Module E := ENV(ValueM)(VarM).
+Import E.
+
+Fixpoint subs (e : env) (t : lterm) : lterm :=
+  match t with
+    | lvar v =>
+      match E.lookup v e with
+        | None => lvar v
+        | Some t => t
+      end
+    | lnode n ts => lnode n (map (subs e) ts)
+  end.
+
+Fixpoint convert (t : lterm) : term :=
+  let converts := fix converts (ts : list lterm) : term :=
+    match ts with
+      | nil => empty
+      | t :: ts => cons (convert t) (converts ts)
+    end in
+  match t with
+    | lvar v => tvar v
+    | lnode n ts => cons (const n) (converts ts)
+  end.
+
+Fixpoint subs' (e : env) (t : term) : term :=
+  match t with
+    | tvar v =>
+      match lookup v e with
+        | None => tvar v
+        | Some t => convert t
+      end
+    | const c => const c
+    | empty => empty
+    | cons p t2 => cons (subs' e p) (subs' e t2)
+  end.
+
+Lemma subs_convert_comm : forall e t,
+  convert (subs e t) = subs' e (convert t).
+Proof.
+  intros.
+  induction t; auto.
+  Case "lvar v".
+    intros. simpl. destruct (lookup v e); auto.
+  Case "node n t::ts".
+    intros. simpl in *. rewrite IHt.
+    inversion IHt0. rewrite H0. reflexivity.
+Qed.
+
+Lemma convert_cons : forall n n' p ps q qs,
+  convert (lnode n (p :: ps)) = convert (lnode n' (q :: qs)) ->
+  n = n' /\ convert p = convert q /\ convert (lnode n ps) = convert (lnode n qs).
+Proof.
+  intros. inversion H. simpl. rewrite H3. auto.
+Qed.
+
+Lemma convert_inj : forall p q,
+  convert p = convert q -> p = q.
+Proof.
+  induction p as [v | n | n p ps IHp IHps]; intros.
+  Case "lvar v".
+    simpl in *. destruct q; inversion H. reflexivity.
+  Case "node n nil".
+    destruct q; inversion H. destruct l; [reflexivity | discriminate H2].
+  Case "node n t::ts".
+    induction q as [ | | n' q qs _ _]; try discriminate H.
+    apply convert_cons in H. inversion_clear H as (N & P & Ps).
+    apply IHp in P. apply IHps in Ps.
+    rewrite N. rewrite P. inversion Ps. reflexivity.
+Qed.
+
+(* Since terms behave the same way under substitution as lterms,
+   we might as well use terms in place of them for convenience. *)
+Lemma conversion_is_faithful: forall (p q : lterm) (e : env),
+  subs e p = subs e q <-> subs' e (convert p) = subs' e (convert q).
+Proof.
+  intros. repeat (rewrite <- subs_convert_comm). split; intros.
+  Case "->".
+    rewrite H. reflexivity.
+  Case "<-".
+    apply convert_inj in H. exact H.
+Qed.
